theories/semantics/store.v
@@ -7,17 +7,3 @@ From osiris.lang Require Import locations lang.
 (* The store is a map of locations to values. *)
 
 Definition store : Type := gmap loc val.
-
-(* [store_ref] finds a fresh location to add to its argument.
- * It returns the fresh location and the updated store. *)
-Definition store_ref (s: store) (v: val) : loc * store :=
-  let l := fresh_loc (dom s) in
-  (l, <[l := v]>s).
-
-Lemma store_ref_dom (s: store) (v: val) :
-  let '(l, s') := store_ref s v in
-  dom s' = (dom s) ∪ {[ l ]} ∧ l ∉ dom s.
-Proof.
-  split; first set_solver.
-  apply fresh_loc_fresh.
-Qed.
